Update invariant

src/invariant/PFCertify.v
@@ -1,4 +1,3 @@
-Require Import Omega.
 Require Import RelationClasses.
 Require Import Coq.Lists.ListDec Decidable.
 
@@ -8,10 +7,10 @@ From PromisingLib Require Import Axioms.
 From PromisingLib Require Import Basic.
 From PromisingLib Require Import DataStructure.
 From PromisingLib Require Import Loc.
+From PromisingLib Require Import Language.
 
 Require Import Time.
 Require Import Event.
-From PromisingLib Require Import Language.
 Require Import View.
 Require Import Cell.
 Require Import Memory.
@@ -34,1188 +33,35 @@ Set Implicit Arguments.
 
 
 Module PFCertify.
-  Include PFCommon.
-
-  Definition cap_src (latests: TimeMap.t) (loc: Loc.t) (promises: Memory.t)
-                     (from: Time.t) (val: Const.t) (released: option View.t):
-    option (Time.t * Message.t) :=
-    if Memory.get loc (latests loc) promises
-    then None
-    else Some (from, Message.concrete val released).
-
-  Inductive sim_memory (latests: TimeMap.t) (caps: Loc.t -> option Time.t) (promises mem_src mem_tgt: Memory.t): Prop :=
-  | sim_memory_intro
-      (SOUND: Memory.le mem_src mem_tgt)
-      (COMPLETE1: forall loc to from msg
-                   (CAP: Some to <> caps loc)
-                   (GETP: Memory.get loc to promises = Some (from, msg))
-                   (GET_TGT: Memory.get loc to mem_tgt = Some (from, msg)),
-          <<GET_SRC: Memory.get loc to mem_src = None>>)
-      (COMPLETE2: forall loc to from msg
-                   (CAP: Some to <> caps loc)
-                   (GETP: Memory.get loc to promises = None)
-                   (GET_TGT: Memory.get loc to mem_tgt = Some (from, msg)),
-          <<GET_SRC: Memory.get loc to mem_src = Some (from, msg)>>)
-      (LATESTS: forall loc to (CAP: Some to = caps loc), Time.lt (latests loc) to)
-      (CAPS: forall loc to (CAP: Some to = caps loc),
-          exists f val r from released,
-            <<LATEST: Memory.get loc (latests loc) mem_tgt = Some (f, Message.concrete val r)>> /\
-            <<CAP_SRC: Memory.get loc to mem_src = cap_src latests loc promises from val released>> /\
-            <<CAP_TGT: Memory.get loc to mem_tgt = Some (from, Message.concrete val released)>> /\
-            <<CAPP: Memory.get loc to promises = None>>)
-  .
-
-  Inductive sim_thread (lang: language) (latests: TimeMap.t) (caps: Loc.t -> option Time.t) (e_src e_tgt: @Thread.t lang): Prop :=
-  | sim_thread_intro
-      (STATE: e_src.(Thread.state) = e_tgt.(Thread.state))
-      (LOCAL: sim_local e_src.(Thread.local) e_tgt.(Thread.local))
-      (SC: e_src.(Thread.sc) = e_tgt.(Thread.sc))
-      (MEMORY: sim_memory latests caps
-                          e_tgt.(Thread.local).(Local.promises)
-                          e_src.(Thread.memory) e_tgt.(Thread.memory))
-  .
-
-
-  Lemma opt_ts_eq_dec (lhs rhs: option Time.t): {lhs = rhs} + {lhs <> rhs}.
-  Proof.
-    destruct lhs, rhs; eauto.
-    - destruct (Time.eq_dec t t0); subst; eauto.
-      right. ii. inv H. ss.
-    - right. ii. ss.
-    - right. ii. ss.
-  Qed.
-
-  Lemma sim_memory_get
-        latests caps promises mem_src mem_tgt
-        loc from to msg
-        (MEM: sim_memory latests caps promises mem_src mem_tgt)
-        (LE_TGT: Memory.le promises mem_tgt)
-        (GET_TGT: Memory.get loc to mem_tgt = Some (from, msg)):
-    <<GETP: Memory.get loc to promises = Some (from, msg)>> /\
-    <<GET_SRC: Memory.get loc to mem_src = None>> \/
-    <<GETP: Memory.get loc to promises = None>> /\
-    <<GET_SRC: Memory.get loc to mem_src = Some (from, msg)>> \/
-    <<TO: Some to = caps loc>> /\
-    <<GETP: Memory.get loc (latests loc) promises>> /\
-    <<GET_SRC: Memory.get loc to mem_src = None>>.
-  Proof.
-    inv MEM.
-    destruct (opt_ts_eq_dec (Some to) (caps loc)).
-    - exploit CAPS; eauto. i. des.
-      unfold cap_src in *.
-      destruct (Memory.get loc (latests loc) promises) as [[]|] eqn:LATESTP.
-      + right. right. exploit LE_TGT; eauto.
-      + right. left.
-        rewrite GET_TGT in *. inv CAP_TGT.
-        splits; auto.
-    - destruct (Memory.get loc to promises) as [[]|] eqn:GETP.
-      + exploit LE_TGT; eauto. i.
-        rewrite GET_TGT in x. inv x. eauto.
-      + exploit COMPLETE2; eauto.
-  Qed.
-
-
-  (* lemmas on step *)
-
-  Lemma promise
-        latests caps mem1_src
-        promises1 mem1_tgt loc from to msg promises2 mem2_tgt kind
-        (MEM1: sim_memory latests caps promises1 mem1_src mem1_tgt)
-        (LE1_TGT: Memory.le promises1 mem1_tgt)
-        (PROMISE_TGT: Memory.promise promises1 mem1_tgt loc from to msg promises2 mem2_tgt kind):
-    sim_memory latests caps promises2 mem1_src mem2_tgt.
-  Proof.
-    inv MEM1. inv PROMISE_TGT.
-    - (* add *)
-      clear TS RESERVE.
-      exploit Memory.add_get0; try exact PROMISES. i. des.
-      exploit Memory.add_get0; try exact MEM. i. des.
-      econs; ii.
-      + erewrite Memory.add_o; eauto. condtac; ss; eauto.
-        des. subst. exploit SOUND; eauto. congr.
-      + revert GETP.
-        erewrite Memory.add_o; eauto. condtac; ss; eauto. i.
-        des. subst.
-        destruct (Memory.get loc to mem1_src) as [[]|] eqn:GET_SRC; ss.
-        exploit SOUND; eauto. congr.
-      + revert GETP.
-        erewrite Memory.add_o; eauto. condtac; ss; eauto. i.
-        revert GET_TGT.
-        erewrite Memory.add_o; eauto. condtac; ss; eauto.
-      + auto.
-      + exploit CAPS; eauto. i. des.
-        erewrite Memory.add_o; eauto. condtac; ss.
-        { des. subst. congr. }
-        esplits; eauto.
-        * unfold cap_src in *. des_ifs; eauto.
-          { revert Heq.
-            erewrite Memory.add_o; eauto. condtac; ss. congr. }
-          { revert Heq.
-            erewrite Memory.add_o; eauto. condtac; ss. congr. }
-        * erewrite Memory.add_o; eauto. condtac; ss.
-          des; subst; congr.
-        * erewrite Memory.add_o; eauto. condtac; ss.
-          des; subst; congr.
-    - (* split *)
-      clear TS RESERVE.
-      exploit Memory.split_get0; try exact PROMISES. i. des.
-      exploit Memory.split_get0; try exact MEM. i. des.
-      econs; ii.
-      + erewrite Memory.split_o; eauto. repeat condtac; ss; eauto.
-        * des. subst. exploit SOUND; eauto. congr.
-        * guardH o. des. subst.
-          exploit COMPLETE1; try exact GET0; eauto; try congr.
-          ii. exploit CAPS; eauto. i. des. congr.
-      + revert GETP.
-        erewrite Memory.split_o; eauto. repeat condtac; ss; eauto; i.
-        * des. subst.
-          destruct (Memory.get loc to mem1_src) as [[]|] eqn:GET_SRC; ss.
-          exploit SOUND; eauto. congr.
-        * guardH o. des. subst. inv GETP. eauto.
-      + revert GETP.
-        erewrite Memory.split_o; eauto. repeat condtac; ss; eauto; i.
-        revert GET_TGT.
-        erewrite Memory.split_o; eauto. repeat condtac; ss; eauto.
-      + auto.
-      + exploit CAPS; eauto. i. des.
-        erewrite Memory.split_o; eauto. repeat condtac; ss.
-        * des. subst. congr.
-        * guardH o. des. subst.
-          rewrite GET4 in *. inv LATEST.
-          esplits; eauto.
-          { unfold cap_src in *. des_ifs; eauto. }
-          { erewrite Memory.split_o; eauto. repeat condtac; [| |eauto]; ss.
-            - des; subst; congr.
-            - des; subst; congr. }
-          { erewrite Memory.split_o; eauto. repeat condtac; ss.
-            - des; subst; congr.
-            - des; subst; congr. }
-        * guardH o. guardH o0.
-          esplits; eauto.
-          { unfold cap_src in *. des_ifs; eauto.
-            - revert Heq.
-              erewrite Memory.split_o; eauto. repeat condtac; ss. congr.
-            - revert Heq.
-              erewrite Memory.split_o; eauto. repeat condtac; ss. congr. }
-          { erewrite Memory.split_o; eauto. repeat condtac; [| |eauto]; ss.
-            - des; subst; congr.
-            - des; subst; congr. }
-          { erewrite Memory.split_o; eauto. repeat condtac; ss.
-            - des; subst; congr.
-            - des; subst; congr. }
-    - (* lower *)
-      clear TS.
-      exploit Memory.lower_get0; try exact PROMISES. i. des.
-      exploit Memory.lower_get0; try exact MEM. i. des.
-      econs; ii.
-      + erewrite Memory.lower_o; eauto. condtac; ss; eauto.
-        des. subst. exploit COMPLETE1; eauto; try congr.
-        ii. exploit CAPS; eauto. i. des. congr.
-      + revert GETP.
-        erewrite Memory.lower_o; eauto. condtac; ss; eauto. i.
-        des. subst. inv GETP.
-        revert GET_TGT.
-        erewrite Memory.lower_o; eauto.
-      + revert GETP.
-        erewrite Memory.lower_o; eauto. condtac; ss; eauto. i.
-        revert GET_TGT.
-        erewrite Memory.lower_o; eauto. condtac; ss; eauto.
-      + auto.
-      + exploit CAPS; eauto. i. des.
-        erewrite Memory.lower_o; eauto. condtac; ss.
-        * des. subst.
-          rewrite GET1 in *. inv LATEST. inv MSG_LE.
-          esplits; eauto.
-          { unfold cap_src in *. des_ifs; eauto. }
-          { erewrite Memory.lower_o; eauto. condtac; [|eauto]; ss.
-            des. subst. congr. }
-          { erewrite Memory.lower_o; eauto. condtac; [|eauto]; ss.
-            des. subst. congr. }
-        * guardH o. esplits; eauto.
-          { unfold cap_src in *. des_ifs; eauto.
-            - revert Heq.
-              erewrite Memory.lower_o; eauto. condtac; ss. congr.
-            - revert Heq.
-              erewrite Memory.lower_o; eauto. condtac; ss. congr. }
-          { erewrite Memory.lower_o; eauto. condtac; [|eauto]; ss.
-            des. subst. congr. }
-          { erewrite Memory.lower_o; eauto. condtac; [|eauto]; ss.
-            des. subst. congr. }
-    - (* cancel *)
-      exploit Memory.remove_get0; try exact PROMISES. i. des.
-      exploit Memory.remove_get0; try exact MEM. i. des.
-      econs; ii.
-      + erewrite Memory.remove_o; eauto. condtac; ss; eauto.
-        des. subst. exploit COMPLETE1; eauto; try congr.
-        ii. exploit CAPS; eauto. i. des. congr.
-      + revert GETP.
-        erewrite Memory.remove_o; eauto. condtac; ss; eauto.
-      + revert GETP.
-        erewrite Memory.remove_o; eauto. condtac; ss; i.
-        * revert GET_TGT.
-          erewrite Memory.remove_o; eauto. condtac; ss; eauto.
-        * revert GET_TGT.
-          erewrite Memory.remove_o; eauto. condtac; ss; eauto.
-      + auto.
-      + exploit CAPS; eauto. i. des.
-        erewrite Memory.remove_o; eauto. condtac; ss.
-        * des. subst.
-          rewrite GET1 in *. inv LATEST.
-        * guardH o. esplits; eauto.
-          { unfold cap_src in *. des_ifs; eauto.
-            - revert Heq.
-              erewrite Memory.remove_o; eauto. condtac; ss. congr.
-            - revert Heq.
-              erewrite Memory.remove_o; eauto. condtac; ss. congr. }
-          { erewrite Memory.remove_o; eauto. condtac; [|eauto]; ss.
-            des. subst. congr. }
-          { erewrite Memory.remove_o; eauto. condtac; [|eauto]; ss. }
-  Qed.
-
-  Lemma read_cap
-        latests caps mem1_src
-        lc1 mem1_tgt loc to val released ord lc2
-        (MEM1: sim_memory latests caps lc1.(Local.promises) mem1_src mem1_tgt)
-        (WF1: Local.wf lc1 mem1_tgt)
-        (TO: Some to = caps loc)
-        (STEP: Local.read_step lc1 mem1_tgt loc to val released ord lc2)
-        (CONS: Local.promise_consistent lc2):
-    Memory.get loc (latests loc) lc1.(Local.promises) = None.
-  Proof.
-    destruct (Memory.get loc (latests loc) (Local.promises lc1)) as [[]|] eqn:PROMISE; ss.
-    exfalso. destruct t0; cycle 1.
-    { inv MEM1. exploit CAPS; eauto. i. des.
-      inv WF1. exploit PROMISES; eauto. i. congr. }
-    inv STEP. exploit CONS; eauto. i.
-    eapply Time.lt_strorder.
-    etrans; eauto.
-    inv MEM1. clear SOUND COMPLETE1 COMPLETE2 CAPS.
-    exploit (LATESTS loc to); eauto. i.
-    eapply TimeFacts.lt_le_lt; eauto. ss.
-    etrans; [|apply Time.join_l]. etrans; [|apply Time.join_r].
-    unfold View.singleton_ur_if. condtac; ss.
-    - unfold TimeMap.singleton.
-      exploit LocFun.add_spec_eq. unfold LocFun.find. i.
-      rewrite x2. refl.
-    - unfold TimeMap.singleton.
-      exploit LocFun.add_spec_eq. unfold LocFun.find. i.
-      rewrite x2. refl.
-  Qed.
-
-  Lemma read_step
-        latests caps
-        lc1_src mem1_src
-        lc1_tgt mem1_tgt loc to val released ord lc2_tgt
-        (LOCAL1: sim_local lc1_src lc1_tgt)
-        (MEM1: sim_memory latests caps lc1_tgt.(Local.promises) mem1_src mem1_tgt)
-        (WF1_TGT: Local.wf lc1_tgt mem1_tgt)
-        (STEP_TGT: Local.read_step lc1_tgt mem1_tgt loc to val released ord lc2_tgt)
-        (CONS_TGT: Local.promise_consistent lc2_tgt):
-    exists lc2_src,
-      <<STEP_SRC: Local.read_step lc1_src mem1_src loc to val released ord lc2_src>> /\
-      <<LOCAL2: sim_local lc2_src lc2_tgt>>.
-  Proof.
-    destruct (Memory.get loc to mem1_src) as [[]|] eqn:GET_SRC.
-    { inv MEM1. exploit SOUND; eauto. i.
-      inv STEP_TGT. rewrite GET in *. inv x.
-      destruct lc1_src, lc1_tgt. inv LOCAL1. ss. subst.
-      esplits; econs; eauto.
-    }
-    dup STEP_TGT. inv STEP_TGT0.
-    exploit sim_memory_get; eauto; try apply WF1_TGT. i. des.
-    - exploit promise_consistent_promise_read; eauto. i. timetac.
-    - congr.
-    - exploit read_cap; eauto. i. rewrite x0 in *. ss.
-  Qed.
-
-  Lemma promise_remove
-        latests caps
-        mem1_src loc from to msg mem2_src
-        promises1 mem1_tgt promises2 mem2_tgt kind
-        promises3
-        (MEM1: sim_memory latests caps promises1 mem1_src mem1_tgt)
-        (LE1_TGT: Memory.le promises1 mem1_tgt)
-        (ADD_SRC: Memory.add mem1_src loc from to msg mem2_src)
-        (PROMISE_TGT: Memory.promise promises1 mem1_tgt loc from to msg promises2 mem2_tgt kind)
-        (REMOVE_SRC: Memory.remove promises2 loc from to msg promises3)
-        (TO: to <> latests loc):
-    <<MEM2: sim_memory latests caps promises3 mem2_src mem2_tgt>>.
-  Proof.
-    exploit promise; try exact PROMISE_TGT; eauto. i. inv x0.
-    exploit Memory.add_get0; try exact ADD_SRC. i. des.
-    exploit Memory.remove_get0; eauto. i. des.
-    inv PROMISE_TGT.
-    - (* add *)
-      clear TS RESERVE.
-      exploit MemoryMerge.add_remove; try exact PROMISES; eauto. i. subst.
-      exploit Memory.add_get0; try exact MEM. i. des.
-      econs; ii.
-      + revert LHS.
-        erewrite Memory.add_o; eauto. condtac; ss; eauto. i.
-        des. subst. inv LHS. ss.
-      + erewrite Memory.add_o; eauto. condtac; ss.
-        * des. subst. congr.
-        * revert GET_TGT.
-          erewrite Memory.add_o; eauto. condtac; ss. i.
-          inv MEM1. eauto.
-      + erewrite Memory.add_o; eauto. condtac; ss.
-        * des. subst. congr.
-        * revert GET_TGT.
-          erewrite Memory.add_o; eauto. condtac; ss. i.
-          inv MEM1. eauto.
-      + auto.
-      + exploit CAPS; eauto. i. des.
-        esplits; eauto.
-        * unfold cap_src in *. des_ifs; eauto.
-          { revert Heq.
-            erewrite Memory.remove_o; eauto. condtac; ss. i.
-            erewrite Memory.add_o; eauto. condtac; ss.
-            guardH o. des. subst. congr. }
-          { revert Heq.
-            erewrite Memory.remove_o; eauto. condtac; ss. i.
-            erewrite Memory.add_o; eauto. condtac; ss; try congr. }
-          { revert Heq.
-            erewrite Memory.remove_o; eauto. condtac; ss; i.
-            - des. subst.
-              erewrite Memory.add_o; eauto. condtac; ss; try congr.
-            - guardH o.
-              erewrite Memory.add_o; eauto. condtac; ss; try congr. }
-          { revert Heq.
-            erewrite Memory.remove_o; eauto. condtac; ss; i.
-            - des. subst. congr.
-            - erewrite Memory.add_o; eauto. condtac; ss.
-              guardH o. des. subst. congr. }
-        * erewrite Memory.remove_o; eauto. condtac; ss.
-    - (* SPLIT *)
-      clear TS RESERVE.
-      exploit Memory.split_get0; try exact PROMISES. i. des.
-      exploit Memory.split_get0; try exact MEM. i. des.
-      econs; ii.
-      + erewrite Memory.split_o; eauto. repeat condtac; ss; i.
-        * des. subst. rewrite GET0 in *. inv LHS. ss.
-        * guardH o. des. subst.
-          revert LHS.
-          erewrite Memory.add_o; eauto. condtac; ss. i.
-          exploit SOUND; try exact LHS. i.
-          rewrite x in *. ss.
-        * revert LHS.
-          erewrite Memory.add_o; eauto. condtac; ss. i.
-          inv MEM1. eauto.
-      + revert GETP.
-        erewrite Memory.remove_o; eauto. condtac; ss; i.
-        erewrite Memory.add_o; eauto. condtac; ss. eauto.
-      + revert GETP.
-        erewrite Memory.remove_o; eauto. condtac; ss; i.
-        * des. subst.
-          erewrite Memory.add_o; eauto. condtac; ss.
-          rewrite GET_TGT in *. ss.
-        * erewrite Memory.add_o; eauto. condtac; ss. eauto.
-      + auto.
-      + exploit CAPS; eauto. i. des.
-        esplits; eauto.
-        * unfold cap_src in *. des_ifs; eauto.
-          { revert Heq.
-            erewrite Memory.remove_o; eauto. condtac; ss. i.
-            erewrite Memory.add_o; eauto. condtac; ss.
-            guardH o. des. subst. congr. }
-          { revert Heq.
-            erewrite Memory.remove_o; eauto. condtac; ss. i.
-            erewrite Memory.add_o; eauto. condtac; ss; try congr. }
-          { revert Heq.
-            erewrite Memory.remove_o; eauto. condtac; ss; i.
-            - des. subst.
-              erewrite Memory.add_o; eauto. condtac; ss; try congr.
-            - guardH o.
-              erewrite Memory.add_o; eauto. condtac; ss; try congr. }
-          { revert Heq.
-            erewrite Memory.remove_o; eauto. condtac; ss; i.
-            - des. subst. congr.
-            - erewrite Memory.add_o; eauto. condtac; ss.
-              guardH o. des. subst. congr. }
-        * erewrite Memory.remove_o; eauto. condtac; ss.
-    - (* lower *)
-      clear TS.
-      exploit Memory.lower_get0; try exact PROMISES. i. des.
-      exploit Memory.lower_get0; try exact MEM. i. des.
-      econs; ii.
-      + revert LHS.
-        erewrite Memory.add_o; eauto. condtac; ss; eauto. i.
-        des. subst. inv LHS. ss.
-      + erewrite Memory.add_o; eauto. condtac; ss.
-        * des. subst. congr.
-        * revert GET_TGT.
-          erewrite Memory.lower_o; eauto. condtac; ss. i.
-          revert GETP.
-          erewrite Memory.remove_o; eauto. condtac; ss.
-          erewrite Memory.lower_o; eauto. condtac; ss.
-          inv MEM1. eauto.
-      + revert GETP.
-        erewrite Memory.remove_o; eauto. condtac; ss.
-        * i. des. subst. congr.
-        * erewrite Memory.lower_o; eauto. condtac; ss. i.
-          erewrite Memory.add_o; eauto. condtac; ss.
-          revert GET_TGT.
-          erewrite Memory.lower_o; eauto. condtac; ss.
-          inv MEM1. eauto.
-      + auto.
-      + exploit CAPS; eauto. i. des.
-        esplits; eauto.
-        * unfold cap_src in *. des_ifs; eauto.
-          { revert Heq.
-            erewrite Memory.remove_o; eauto. condtac; ss. i.
-            erewrite Memory.add_o; eauto. condtac; ss.
-            guardH o. des. subst. congr. }
-          { revert Heq.
-            erewrite Memory.remove_o; eauto. condtac; ss. i.
-            erewrite Memory.add_o; eauto. condtac; ss; try congr. }
-          { revert Heq.
-            erewrite Memory.remove_o; eauto. condtac; ss; i.
-            - des. subst.
-              erewrite Memory.add_o; eauto. condtac; ss; try congr.
-            - guardH o.
-              erewrite Memory.add_o; eauto. condtac; ss; try congr. }
-          { revert Heq.
-            erewrite Memory.remove_o; eauto. condtac; ss; i.
-            - des. subst. congr.
-            - erewrite Memory.add_o; eauto. condtac; ss.
-              guardH o. des. subst. congr. }
-        * erewrite Memory.remove_o; eauto. condtac; ss.
-    - (* cancel *)
-      exploit Memory.remove_get0; try exact REMOVE_SRC. i. des.
-      exploit Memory.remove_get0; try exact PROMISES. i. des. congr.
-  Qed.
-
-  Lemma promise_remove_latest_Some
-        latests caps
-        mem1_src loc from val released mem2_src
-        promises1 mem1_tgt promises2 mem2_tgt kind
-        promises3
-        to
-        (MEM1: sim_memory latests caps promises1 mem1_src mem1_tgt)
-        (LE1_TGT: Memory.le promises1 mem1_tgt)
-        (CLOSED1_TGT: Memory.closed mem1_tgt)
-        (ADD_SRC: Memory.add mem1_src loc from (latests loc) (Message.concrete val released) mem2_src)
-        (PROMISE_TGT: Memory.promise promises1 mem1_tgt loc from (latests loc) (Message.concrete val released) promises2 mem2_tgt kind)
-        (REMOVE_SRC: Memory.remove promises2 loc from (latests loc) (Message.concrete val released) promises3)
-        (TO: caps loc = Some to):
-    exists from_cap released_cap mem3_src,
-      <<CAP_TGT: Memory.get loc to mem2_tgt = Some (from_cap, Message.concrete val released_cap)>> /\
-      <<ADD: Memory.add mem2_src loc from_cap to (Message.concrete val released_cap) mem3_src>> /\
-      <<MEM2: sim_memory latests caps promises3 mem3_src mem2_tgt>>.
-  Proof.
-    inv PROMISE_TGT; ss.
-    { (* add *)
-      inv MEM1. exploit CAPS; eauto. i. des.
-      exploit Memory.add_get0; try exact MEM. i. des. congr.
-    }
-    { (* split *)
-      inv MEM1. exploit CAPS; eauto. i. des.
-      exploit Memory.split_get0; try exact MEM. i. des. congr.
-    }
-    (* lower *)
-    clear TS RESERVE.
-    inv MEM1. exploit CAPS; eauto. i. des.
-    exploit Memory.lower_get0; try exact PROMISES. i. des.
-    exploit Memory.lower_get0; try exact MEM. i. des.
-    rewrite GET1 in *. inv LATEST. inv MSG_LE. clear MSG_LE0.
-    unfold cap_src in CAP_SRC. rewrite GET in *.
-    exploit LATESTS; eauto. intro LATEST_LT.
-    exploit (@Memory.add_exists mem2_src loc from0 to (Message.concrete val0 released0)).
-    { ii. revert GET3.
-      erewrite Memory.add_o; eauto. condtac; ss; i.
-      - des. subst. inv GET3.
-        exploit Memory.get_disjoint; [exact CAP_TGT|exact GET1|..]. i. des.
-        + subst. timetac.
-        + eapply x1; eauto.
-      - guardH o. exploit SOUND; eauto. i.
-        exploit Memory.get_disjoint; [exact CAP_TGT|exact x0|..]. i. des.
-        + subst. congr.
-        + eapply x2; eauto. }
-    { exploit Memory.get_ts; try exact CAP_TGT. i. des; ss.
-      subst. exploit LATESTS; eauto. i. inv x. }
-    { inv CLOSED1_TGT. exploit CLOSED; try exact CAP_TGT. i. des. ss. }
-    i. des.
-    erewrite Memory.lower_o; eauto. condtac; ss.
-    { des. subst. timetac. }
-    clear o COND.
-    esplits; eauto.
-    econs; ii.
-    - revert LHS.
-      erewrite Memory.add_o; eauto. condtac; ss.
-      + i. des. subst. inv LHS.
-        erewrite Memory.lower_o; eauto. condtac; ss.
-        des. subst. timetac.
-      + guardH o.
-        erewrite Memory.add_o; eauto. condtac; ss; i.
-        * des. subst. inv LHS. ss.
-        * erewrite Memory.lower_o; eauto. condtac; ss. eauto.
-    - erewrite Memory.add_o; eauto. condtac; ss.
-      + des. subst. congr.
-      + guardH o.
-        erewrite Memory.add_o; eauto. condtac; ss.
-        * des. subst.
-          exploit Memory.remove_get0; eauto. i. des. congr.
-        * revert GETP.
-          erewrite Memory.remove_o; eauto. condtac; ss.
-          erewrite Memory.lower_o; eauto. condtac; ss. i.
-          revert GET_TGT.
-          erewrite Memory.lower_o; eauto.
-    - erewrite Memory.add_o; eauto. condtac; ss.
-      + des. subst. congr.
-      + guardH o.
-        erewrite Memory.add_o; eauto. condtac; ss.
-        * des. subst.
-          exploit Memory.remove_get0; eauto. i. des. congr.
-        * revert GETP.
-          erewrite Memory.remove_o; eauto. condtac; ss.
-          erewrite Memory.lower_o; eauto. condtac; ss. i.
-          revert GET_TGT.
-          erewrite Memory.lower_o; eauto. condtac; ss. i.
-          eauto.
-    - auto.
-    - erewrite Memory.lower_o; eauto. condtac; ss.
-      + des. subst. rewrite TO in *. inv CAP.
-        esplits; eauto.
-        * erewrite Memory.add_o; eauto. condtac; ss.
-          { unfold cap_src.
-            erewrite Memory.remove_o; eauto. condtac; ss.
-            revert COND1. condtac; ss. }
-          { des; ss. }
-        * erewrite Memory.lower_o; eauto. condtac; ss.
-          des. subst. timetac.
-        * erewrite Memory.remove_o; eauto. condtac; ss.
-          erewrite Memory.lower_o; eauto. condtac; ss.
-      + destruct (Loc.eq_dec loc0 loc).
-        { subst. des; ss. }
-        guardH o.
-        exploit CAPS; try exact CAP. i. des.
-        esplits; eauto.
-        * erewrite Memory.add_o; eauto. condtac; ss.
-          { des; subst; ss. }
-          erewrite Memory.add_o; eauto. condtac; ss.
-          { des; subst; ss. }
-          unfold cap_src in *. des_ifs; eauto.
-          { revert Heq.
-            erewrite Memory.remove_o; eauto. condtac; ss.
-            erewrite Memory.lower_o; eauto. condtac; ss.
-            congr. }
-          { revert Heq.
-            erewrite Memory.remove_o; eauto. condtac; ss.
-            erewrite Memory.lower_o; eauto. condtac; ss.
-            congr. }
-        * erewrite Memory.lower_o; eauto. condtac; ss.
-          des. subst. ss.
-        * erewrite Memory.remove_o; eauto. condtac; ss.
-          erewrite Memory.lower_o; eauto. condtac; ss.
-  Qed.
-
-  Lemma promise_remove_latest_None
-        latests caps
-        mem1_src loc from msg mem2_src
-        promises1 mem1_tgt promises2 mem2_tgt kind
-        promises3
-        (MEM1: sim_memory latests caps promises1 mem1_src mem1_tgt)
-        (LE1_TGT: Memory.le promises1 mem1_tgt)
-        (ADD_SRC: Memory.add mem1_src loc from (latests loc) msg mem2_src)
-        (PROMISE_TGT: Memory.promise promises1 mem1_tgt loc from (latests loc) msg promises2 mem2_tgt kind)
-        (REMOVE_SRC: Memory.remove promises2 loc from (latests loc) msg promises3)
-        (TO: caps loc = None):
-    <<MEM2: sim_memory latests caps promises3 mem2_src mem2_tgt>>.
-  Proof.
-    exploit promise; try exact PROMISE_TGT; eauto. i. inv x0.
-    exploit Memory.add_get0; try exact ADD_SRC. i. des.
-    exploit Memory.remove_get0; eauto. i. des.
-    inv PROMISE_TGT.
-    - (* add *)
-      clear TS RESERVE.
-      exploit MemoryMerge.add_remove; try exact PROMISES; eauto. i. subst.
-      exploit Memory.add_get0; try exact MEM. i. des.
-      econs; ii.
-      + revert LHS.
-        erewrite Memory.add_o; eauto. condtac; ss; eauto. i.
-        des. subst. inv LHS. ss.
-      + erewrite Memory.add_o; eauto. condtac; ss.
-        * des. subst. congr.
-        * revert GET_TGT.
-          erewrite Memory.add_o; eauto. condtac; ss. i.
-          inv MEM1. eauto.
-      + erewrite Memory.add_o; eauto. condtac; ss.
-        * des. subst. congr.
-        * revert GET_TGT.
-          erewrite Memory.add_o; eauto. condtac; ss. i.
-          inv MEM1. eauto.
-      + auto.
-      + exploit CAPS; eauto. i. des.
-        esplits; eauto.
-        * unfold cap_src in *. des_ifs; eauto.
-          { revert Heq.
-            erewrite Memory.remove_o; eauto. condtac; ss. i.
-            erewrite Memory.add_o; eauto. condtac; ss.
-            guardH o. des. subst. congr. }
-          { revert Heq.
-            erewrite Memory.remove_o; eauto. condtac; ss. i.
-            erewrite Memory.add_o; eauto. condtac; ss; try congr. }
-          { revert Heq.
-            erewrite Memory.remove_o; eauto. condtac; ss; i.
-            - des. subst. congr.
-            - guardH o.
-              erewrite Memory.add_o; eauto. condtac; ss; try congr. }
-          { revert Heq.
-            erewrite Memory.remove_o; eauto. condtac; ss; i.
-            - des. subst. congr.
-            - erewrite Memory.add_o; eauto. condtac; ss.
-              guardH o. des. subst. congr. }
-        * erewrite Memory.remove_o; eauto. condtac; ss.
-    - (* SPLIT *)
-      clear TS RESERVE.
-      exploit Memory.split_get0; try exact PROMISES. i. des.
-      exploit Memory.split_get0; try exact MEM. i. des.
-      econs; ii.
-      + erewrite Memory.split_o; eauto. repeat condtac; ss; i.
-        * des. subst. rewrite GET0 in *. inv LHS. ss.
-        * guardH o. des. subst.
-          revert LHS.
-          erewrite Memory.add_o; eauto. condtac; ss. i.
-          exploit SOUND; try exact LHS. i.
-          rewrite x in *. ss.
-        * revert LHS.
-          erewrite Memory.add_o; eauto. condtac; ss. i.
-          inv MEM1. eauto.
-      + revert GETP.
-        erewrite Memory.remove_o; eauto. condtac; ss; i.
-        erewrite Memory.add_o; eauto. condtac; ss. eauto.
-      + revert GETP.
-        erewrite Memory.remove_o; eauto. condtac; ss; i.
-        * des. subst.
-          erewrite Memory.add_o; eauto. condtac; ss.
-          rewrite GET_TGT in *. ss.
-        * erewrite Memory.add_o; eauto. condtac; ss. eauto.
-      + auto.
-      + exploit CAPS; eauto. i. des.
-        esplits; eauto.
-        * unfold cap_src in *. des_ifs; eauto.
-          { revert Heq.
-            erewrite Memory.remove_o; eauto. condtac; ss. i.
-            erewrite Memory.add_o; eauto. condtac; ss.
-            guardH o. des. subst. congr. }
-          { revert Heq.
-            erewrite Memory.remove_o; eauto. condtac; ss. i.
-            erewrite Memory.add_o; eauto. condtac; ss; try congr. }
-          { revert Heq.
-            erewrite Memory.remove_o; eauto. condtac; ss; i.
-            - des. subst.
-              erewrite Memory.add_o; eauto. condtac; ss; try congr.
-            - guardH o.
-              erewrite Memory.add_o; eauto. condtac; ss; try congr. }
-          { revert Heq.
-            erewrite Memory.remove_o; eauto. condtac; ss; i.
-            - des. subst. congr.
-            - erewrite Memory.add_o; eauto. condtac; ss.
-              guardH o. des. subst. congr. }
-        * erewrite Memory.remove_o; eauto. condtac; ss.
-    - (* lower *)
-      clear TS.
-      exploit Memory.lower_get0; try exact PROMISES. i. des.
-      exploit Memory.lower_get0; try exact MEM. i. des.
-      econs; ii.
-      + revert LHS.
-        erewrite Memory.add_o; eauto. condtac; ss; eauto. i.
-        des. subst. inv LHS. ss.
-      + erewrite Memory.add_o; eauto. condtac; ss.
-        * des. subst. congr.
-        * revert GET_TGT.
-          erewrite Memory.lower_o; eauto. condtac; ss. i.
-          revert GETP.
-          erewrite Memory.remove_o; eauto. condtac; ss.
-          erewrite Memory.lower_o; eauto. condtac; ss.
-          inv MEM1. eauto.
-      + revert GETP.
-        erewrite Memory.remove_o; eauto. condtac; ss.
-        * i. des. subst. congr.
-        * erewrite Memory.lower_o; eauto. condtac; ss. i.
-          erewrite Memory.add_o; eauto. condtac; ss.
-          revert GET_TGT.
-          erewrite Memory.lower_o; eauto. condtac; ss.
-          inv MEM1. eauto.
-      + auto.
-      + exploit CAPS; eauto. i. des.
-        esplits; eauto.
-        * unfold cap_src in *. des_ifs; eauto.
-          { revert Heq.
-            erewrite Memory.remove_o; eauto. condtac; ss. i.
-            erewrite Memory.add_o; eauto. condtac; ss.
-            guardH o. des. subst. congr. }
-          { revert Heq.
-            erewrite Memory.remove_o; eauto. condtac; ss. i.
-            erewrite Memory.add_o; eauto. condtac; ss; try congr. }
-          { revert Heq.
-            erewrite Memory.remove_o; eauto. condtac; ss; i.
-            - des. subst.
-              erewrite Memory.add_o; eauto. condtac; ss; try congr.
-            - guardH o.
-              erewrite Memory.add_o; eauto. condtac; ss; try congr. }
-          { revert Heq.
-            erewrite Memory.remove_o; eauto. condtac; ss; i.
-            - des. subst. congr.
-            - erewrite Memory.add_o; eauto. condtac; ss.
-              guardH o. des. subst. congr. }
-        * erewrite Memory.remove_o; eauto. condtac; ss.
-    - (* cancel *)
-      exploit Memory.remove_get0; try exact REMOVE_SRC. i. des.
-      exploit Memory.remove_get0; try exact PROMISES. i. des. congr.
-  Qed.
-
-  Lemma write_aux
-        latests caps
-        mem1_src
-        lc1_tgt sc1 mem1_tgt loc from to val releasedm released ord lc2_tgt sc2 mem2_tgt kind
-        (MEM1: sim_memory latests caps lc1_tgt.(Local.promises) mem1_src mem1_tgt)
-        (WF1_TGT: Local.wf lc1_tgt mem1_tgt)
-        (RELEASEDM: View.opt_wf releasedm)
-        (STEP_TGT: Local.write_step lc1_tgt sc1 mem1_tgt loc from to val
-                                    releasedm released ord lc2_tgt sc2 mem2_tgt kind):
-    exists mem2_src,
-      Memory.add mem1_src loc from to
-                 (Message.concrete val (TView.write_released (Local.tview lc1_tgt) sc1 loc to releasedm ord)) mem2_src.
-  Proof.
-    inv STEP_TGT. inv WRITE.
-    exploit (@Memory.add_exists mem1_src loc from to
-                                (Message.concrete val (TView.write_released (Local.tview lc1_tgt) sc1 loc to releasedm ord))); eauto.
-    { inv MEM1. inv PROMISE; ss; ii.
-      - clear TS RESERVE.
-        exploit SOUND; eauto. i.
-        exploit Memory.add_get1; eauto. i.
-        exploit Memory.add_get0; try exact MEM. i. des.
-        exploit Memory.get_disjoint; [exact x2|exact GET0|..]. i. des.
-        + subst.
-          exploit Memory.add_get0; try exact PROMISES. i. des.
-          exploit COMPLETE2; try exact GET1; eauto.
-          { ii. exploit CAPS; eauto. i. des. congr. }
-          i. des. congr.
-        + eapply x3; eauto.
-      - clear TS RESERVE.
-        exploit SOUND; eauto. i.
-        exploit Memory.split_get0; eauto. i. des.
-        exploit Memory.get_disjoint; [exact x0|exact GET0|..]. i. des.
-        + subst.
-          exploit Memory.split_get0; try exact PROMISES. i. des.
-          exploit COMPLETE1; try exact GET5; eauto.
-          { ii. exploit CAPS; eauto. i. des. congr. }
-          i. des. congr.
-        + eapply x2; eauto.
-          inv LHS. ss. econs; ss.
-          etrans; eauto. econs.
-          inv MEM. inv SPLIT. ss.
-      - clear TS.
-        exploit SOUND; eauto. i.
-        exploit Memory.lower_get0; try exact MEM. i. des.
-        exploit Memory.get_disjoint; [exact x0|exact GET|..]. i. des.
-        + subst.
-          exploit Memory.lower_get0; try exact PROMISES. i. des.
-          exploit COMPLETE1; try exact GET1; eauto.
-          { ii. exploit CAPS; eauto. i. des. congr. }
-          i. des. congr.
-        + eapply x2; eauto.
-    }
-    { inv PROMISE; ss.
-      - inv MEM. inv ADD. ss.
-      - inv MEM. inv SPLIT. ss.
-      - inv MEM. inv LOWER. ss.
-    }
-    { inv PROMISE; ss.
-      - inv MEM. inv ADD. ss.
-      - inv MEM. inv SPLIT. ss.
-      - inv MEM. inv LOWER. ss.
-    }
-  Qed.
-
-  Lemma write_step
-        latests caps
-        lc1_src mem1_src
-        lc1_tgt sc1 mem1_tgt loc from to val releasedm released ord lc2_tgt sc2 mem2_tgt kind
-        (LOCAL1: sim_local lc1_src lc1_tgt)
-        (MEM1: sim_memory latests caps lc1_tgt.(Local.promises) mem1_src mem1_tgt)
-        (WF1_TGT: Local.wf lc1_tgt mem1_tgt)
-        (RELEASEDM: View.opt_wf releasedm)
-        (STEP_TGT: Local.write_step lc1_tgt sc1 mem1_tgt loc from to val
-                                    releasedm released ord lc2_tgt sc2 mem2_tgt kind)
-        (TO: to <> latests loc):
-    exists lc2_src mem2_src,
-      <<STEP_SRC: ALocal.write_step lc1_src sc1 mem1_src loc from to val
-                                    releasedm released ord lc2_src sc2 mem2_src Memory.op_kind_add>> /\
-      <<LOCAL2: sim_local lc2_src lc2_tgt>> /\
-      <<MEM2: sim_memory latests caps lc2_tgt.(Local.promises) mem2_src mem2_tgt>>.
-  Proof.
-    exploit write_aux; eauto. i. des.
-    exploit Memory.add_exists_le; try eapply Memory.bot_le; eauto. i. des.
-    exploit Memory.add_get0; try exact x1. i. des.
-    exploit Memory.remove_exists; try exact GET0. i. des.
-    destruct lc1_src, lc1_tgt. ss.
-    inv LOCAL1. inv STEP_TGT. ss. subst.
-    esplits.
-    - econs; ss.
-      + econs; eauto. econs; eauto; ss.
-        inv WRITE. inv PROMISE; ss.
-      + ii. rewrite Memory.bot_get in *. ss.
-    - exploit MemoryMerge.add_remove; eauto.
-    - inv WRITE. eapply promise_remove; eauto. apply WF1_TGT.
-  Qed.
-
-  Lemma write_step_latest_Some
-        latests caps
-        lc1_src mem1_src
-        lc1_tgt sc1 mem1_tgt loc from val releasedm released ord lc2_tgt sc2 mem2_tgt kind
-        to
-        (LOCAL1: sim_local lc1_src lc1_tgt)
-        (MEM1: sim_memory latests caps lc1_tgt.(Local.promises) mem1_src mem1_tgt)
-        (WF1_TGT: Local.wf lc1_tgt mem1_tgt)
-        (CLOSED1_TGT: Memory.closed mem1_tgt)
-        (RELEASEDM: View.opt_wf releasedm)
-        (STEP_TGT: Local.write_step lc1_tgt sc1 mem1_tgt loc from (latests loc) val
-                                    releasedm released ord lc2_tgt sc2 mem2_tgt kind)
-        (CAP: caps loc = Some to):
-    exists lc2_src mem2_src mem3_src from_cap released_cap,
-      <<STEP_SRC: ALocal.write_step lc1_src sc1 mem1_src loc from (latests loc) val
-                                    releasedm released ord lc2_src sc2 mem2_src Memory.op_kind_add>> /\
-      <<ADD: Memory.add mem2_src loc from_cap to (Message.concrete val released_cap) mem3_src>> /\
-      <<LOCAL2: sim_local lc2_src lc2_tgt>> /\
-      <<MEM2: sim_memory latests caps lc2_tgt.(Local.promises) mem3_src mem2_tgt>>.
-  Proof.
-    exploit write_aux; eauto. i. des.
-    exploit Memory.add_exists_le; try eapply Memory.bot_le; eauto. i. des.
-    exploit Memory.add_get0; try exact x1. i. des.
-    exploit Memory.remove_exists; try exact GET0. i. des.
-    destruct lc1_src, lc1_tgt. ss.
-    inv LOCAL1. inv STEP_TGT. inv WRITE. ss. subst.
-    exploit promise_remove_latest_Some; eauto; try apply WF1_TGT. i. des.
-    esplits.
-    - econs; ss.
-      + econs; try exact x2. econs; eauto; ss.
-        inv PROMISE; ss.
-      + ii. rewrite Memory.bot_get in *. ss.
-    - eauto.
-    - econs; eauto. ss.
-      exploit MemoryMerge.add_remove; try exact x1; eauto.
-    - auto.
-  Qed.
-
-  Lemma write_step_latest_None
-        latests caps
-        lc1_src mem1_src
-        lc1_tgt sc1 mem1_tgt loc from val releasedm released ord lc2_tgt sc2 mem2_tgt kind
-        (LOCAL1: sim_local lc1_src lc1_tgt)
-        (MEM1: sim_memory latests caps lc1_tgt.(Local.promises) mem1_src mem1_tgt)
-        (WF1_TGT: Local.wf lc1_tgt mem1_tgt)
-        (RELEASEDM: View.opt_wf releasedm)
-        (STEP_TGT: Local.write_step lc1_tgt sc1 mem1_tgt loc from (latests loc) val
-                                    releasedm released ord lc2_tgt sc2 mem2_tgt kind)
-        (CAP: caps loc = None):
-    exists lc2_src mem2_src,
-      <<STEP_SRC: ALocal.write_step lc1_src sc1 mem1_src loc from (latests loc) val
-                                    releasedm released ord lc2_src sc2 mem2_src Memory.op_kind_add>> /\
-      <<LOCAL2: sim_local lc2_src lc2_tgt>> /\
-      <<MEM2: sim_memory latests caps lc2_tgt.(Local.promises) mem2_src mem2_tgt>>.
-  Proof.
-    exploit write_aux; eauto. i. des.
-    exploit Memory.add_exists_le; try eapply Memory.bot_le; eauto. i. des.
-    exploit Memory.add_get0; try exact x1. i. des.
-    exploit Memory.remove_exists; try exact GET0. i. des.
-    destruct lc1_src, lc1_tgt. ss.
-    inv LOCAL1. inv STEP_TGT. ss. subst.
-    esplits.
-    - econs; ss.
-      + econs; eauto. econs; eauto; ss.
-        inv WRITE. inv PROMISE; ss.
-      + ii. rewrite Memory.bot_get in *. ss.
-    - exploit MemoryMerge.add_remove; eauto.
-    - inv WRITE. eapply promise_remove_latest_None; eauto. apply WF1_TGT.
-  Qed.
-
-  Inductive add_cap (caps: Loc.t -> option Time.t): forall (mem1 mem2: Memory.t), Prop :=
-  | add_cap_refl mem:
-      add_cap caps mem mem
-  | add_cap_add
-      mem1 mem2
-      loc from to val released
-      from_cap to_cap released_cap
-      (GET: Memory.get loc to mem1 = Some (from, Message.concrete val released))
-      (CAPTS: caps loc = Some to_cap)
-      (LOWER: Memory.add mem1 loc from_cap to_cap (Message.concrete val released_cap) mem2):
-      add_cap caps mem1 mem2
-  .
-  Hint Constructors add_cap.
-
-  Program Instance add_cap_Reflexive: forall caps, Reflexive (add_cap caps).
-
-  Inductive pf_step (lang: language) (caps: Loc.t -> option Time.t) (e: ThreadEvent.t):
-    forall (e1 e2: Thread.t lang), Prop :=
-  | pf_step_intro
-      e1 st2 lc2 sc2 mem2 mem3
-      (STEP: @AThread.program_step lang e e1 (Thread.mk lang st2 lc2 sc2 mem2))
-      (ADD: @add_cap caps mem2 mem3):
-      pf_step caps e e1 (Thread.mk lang st2 lc2 sc2 mem3)
-  .
-  Hint Constructors pf_step.
-
-  Lemma add_cap_vals_incl
-        caps mem1 mem2
-        (ADD: add_cap caps mem1 mem2):
-    vals_incl mem2 mem1.
-  Proof.
-    inv ADD; try refl. ii. revert GET1.
-    erewrite Memory.add_o; eauto. condtac; ss; eauto. i.
-    des. subst. inv GET1. eauto.
-  Qed.
-
-  Lemma pf_step_inhabited
-        lang caps e e1 e2
-        (STEP: @pf_step lang caps e e1 e2)
-        (INHABITED1: Memory.inhabited e1.(Thread.memory)):
-    <<INHABITED2: Memory.inhabited e2.(Thread.memory)>>.
-  Proof.
-    inv STEP.
-    hexploit AThread.program_step_inhabited; eauto. i.
-    inv ADD; ss.
-    eapply Memory.add_inhabited; eauto.
-  Qed.
-
-  Lemma program_step
-        latests caps
-        lc1_src mem1_src
-        e lc1_tgt sc1 mem1_tgt lc2_tgt sc2 mem2_tgt
-        (LOCAL1: sim_local lc1_src lc1_tgt)
-        (MEM1: sim_memory latests caps lc1_tgt.(Local.promises) mem1_src mem1_tgt)
-        (WF1_TGT: Local.wf lc1_tgt mem1_tgt)
-        (SC1_TGT: Memory.closed_timemap sc1 mem1_tgt)
-        (CLOSED1_TGT: Memory.closed mem1_tgt)
-        (STEP_TGT: Local.program_step e lc1_tgt sc1 mem1_tgt lc2_tgt sc2 mem2_tgt)
-        (CONS: Local.promise_consistent lc2_tgt):
-    exists lc2_src mem2_src mem3_src,
-      <<STEP_SRC: ALocal.program_step e lc1_src sc1 mem1_src lc2_src sc2 mem2_src>> /\
-      <<ADD: add_cap caps mem2_src mem3_src>> /\
-      <<LOCAL2: sim_local lc2_src lc2_tgt>> /\
-      <<MEM2: sim_memory latests caps lc2_tgt.(Local.promises) mem3_src mem2_tgt>>.
-  Proof.
-    inv STEP_TGT.
-    - esplits; eauto.
-    - exploit read_step; eauto. i. des.
-      esplits; try exact LOCAL2; eauto.
-      inv LOCAL. ss.
-    - destruct (Time.eq_dec to (latests loc)).
-      + destruct (caps loc) as [c|] eqn:CAPTS.
-        * subst. exploit write_step_latest_Some; try exact LOCAL; eauto. i. des.
-          esplits; try exact LOCAL2; try exact MEM2; eauto.
-          inv STEP_SRC.
-          exploit AMemory.write_get2; eauto. i. des. eauto.
-        * subst. exploit write_step_latest_None; try exact LOCAL; eauto. i. des.
-          esplits; try exact LOCAL2; eauto.
-      + exploit write_step; try exact LOCAL; eauto. i. des.
-        esplits; try exact LOCAL2; eauto.
-    - exploit read_step; eauto.
-      { eapply write_step_promise_consistent; eauto. }
-      i. des.
-      exploit Local.read_step_future; try exact LOCAL0; eauto. i. des.
-      destruct (Time.eq_dec tsw (latests loc)).
-      + destruct (caps loc) as [c|] eqn:CAPTS.
-        * subst. exploit write_step_latest_Some; try exact LOCAL2; eauto.
-          { inv LOCAL0. eauto. }
-          i. des.
-          esplits; try exact LOCAL4; try exact MEM2; eauto.
-          inv STEP_SRC0.
-          exploit AMemory.write_get2; eauto. i. des. eauto.
-        * subst. exploit write_step_latest_None; try exact LOCAL2; eauto.
-          { inv LOCAL0. eauto. }
-          i. des.
-          esplits; try exact LOCAL4; eauto.
-      + exploit write_step; try exact LOCAL2; eauto.
-        { inv LOCAL0. eauto. }
-        i. des.
-        esplits; try exact LOCAL4; eauto.
-    - exploit fence_step; eauto. i. des.
-      esplits; try exact LOCAL2; eauto.
-      inv LOCAL. ss.
-    - exploit fence_step; eauto. i. des.
-      esplits; try exact LOCAL2; eauto.
-      inv LOCAL. ss.
-    - exploit failure_step; eauto. i. des.
-      esplits; eauto.
-  Qed.
-
-  Lemma thread_promise_step
-        lang latests caps e1_src
-        pf e e1_tgt e2_tgt
-        (SIM1: @sim_thread lang latests caps e1_src e1_tgt)
-        (WF1_TGT: Local.wf e1_tgt.(Thread.local) e1_tgt.(Thread.memory))
-        (MEM1_TGT: Memory.closed e1_tgt.(Thread.memory))
-        (STEP_TGT: Thread.promise_step pf e e1_tgt e2_tgt):
-    sim_thread latests caps e1_src e2_tgt.
-  Proof.
-    destruct e1_src, e1_tgt, e2_tgt. ss.
-    inv SIM1. inv LOCAL. inv STEP_TGT. ss. subst.
-    destruct local, local0; ss. subst.
-    inv LOCAL.
-    econs; ss; eauto.
-    eapply promise; eauto. apply WF1_TGT.
-  Qed.
-
-  Lemma thread_program_step
-        lang latests caps e1_src
-        e e1_tgt e2_tgt
-        (SIM1: @sim_thread lang latests caps e1_src e1_tgt)
-        (WF1_TGT: Local.wf e1_tgt.(Thread.local) e1_tgt.(Thread.memory))
-        (SC1_TGT: Memory.closed_timemap e1_tgt.(Thread.sc) e1_tgt.(Thread.memory))
-        (MEM1_TGT: Memory.closed e1_tgt.(Thread.memory))
-        (STEP_TGT: Thread.program_step e e1_tgt e2_tgt)
-        (CONS: Local.promise_consistent e2_tgt.(Thread.local)):
-    exists e2_src,
-      <<STEP_SRC: pf_step caps e e1_src e2_src>> /\
-      <<SIM2: sim_thread latests caps e2_src e2_tgt>>.
-  Proof.
-    destruct e1_src, e1_tgt, e2_tgt. ss.
-    inv SIM1. inv STEP_TGT. ss. subst.
-    exploit program_step; try exact LOCAL; try exact MEMORY; eauto. i. des.
-    esplits; eauto.
-    - econs; eauto. econs; eauto.
-    - econs; ss.
-  Qed.
-
-  Lemma thread_rtc_all_step
-        lang latests caps e1_src
-        e1_tgt e2_tgt
-        (SIM1: @sim_thread lang latests caps e1_src e1_tgt)
-        (WF1_TGT: Local.wf e1_tgt.(Thread.local) e1_tgt.(Thread.memory))
-        (SC1_TGT: Memory.closed_timemap e1_tgt.(Thread.sc) e1_tgt.(Thread.memory))
-        (MEM1_TGT: Memory.closed e1_tgt.(Thread.memory))
-        (STEPS_TGT: rtc (@Thread.all_step lang) e1_tgt e2_tgt)
-        (CONS: Local.promise_consistent e2_tgt.(Thread.local)):
-    exists e2_src,
-      <<STEPS_SRC: rtc (union (@pf_step lang caps)) e1_src e2_src>> /\
-      <<SIM2: sim_thread latests caps e2_src e2_tgt>>.
-  Proof.
-    revert e1_src SIM1.
-    induction STEPS_TGT; eauto; i.
-    inv H. inv USTEP.
-    exploit Thread.step_future; eauto. i. des.
-    inv STEP.
-    - exploit thread_promise_step; eauto.
-    - exploit thread_program_step; eauto.
-      { eapply rtc_all_step_promise_consistent; eauto. }
-      i. des.
-      exploit IHSTEPS_TGT; eauto. i. des.
-      esplits; try exact SIM0.
-      econs 2; eauto.
-  Qed.
-
-  Lemma thread_rtc_tau_step
-        lang latests caps e1_src
-        e1_tgt e2_tgt
-        (SIM1: @sim_thread lang latests caps e1_src e1_tgt)
-        (WF1_TGT: Local.wf e1_tgt.(Thread.local) e1_tgt.(Thread.memory))
-        (SC1_TGT: Memory.closed_timemap e1_tgt.(Thread.sc) e1_tgt.(Thread.memory))
-        (MEM1_TGT: Memory.closed e1_tgt.(Thread.memory))
-        (STEPS_TGT: rtc (@Thread.tau_step lang) e1_tgt e2_tgt)
-        (CONS: Local.promise_consistent e2_tgt.(Thread.local)):
-    exists e2_src,
-      <<STEPS_SRC: rtc (union (@pf_step lang caps)) e1_src e2_src>> /\
-      <<SIM2: sim_thread latests caps e2_src e2_tgt>>.
-  Proof.
-    eapply thread_rtc_all_step; eauto.
-    eapply rtc_implies; [|eauto].
-    apply tau_union.
-  Qed.
-
+  Include PFStep.
 
   (* existence of sim *)
 
-  Definition cap_src_cell (latest: Time.t) (promises: Cell.t)
-                          (from: Time.t) (val: Const.t) (released: option View.t):
-    option (Time.t * Message.t) :=
-    if Cell.get latest promises
-    then None
-    else Some (from, Message.concrete val released).
-
-  Inductive sim_cell (latest: Time.t) (cap: option Time.t) (promises cell_src cell_tgt: Cell.t): Prop :=
+  Inductive sim_cell (promises cell_src cell_tgt: Cell.t): Prop :=
   | sim_cell_intro
-      (LATEST: exists from val released,
-          Cell.get latest cell_tgt = Some (from, Message.concrete val released))
       (SOUND: Cell.le cell_src cell_tgt)
       (COMPLETE1: forall to from msg
-                   (CAP: Some to <> cap)
                    (GETP: Cell.get to promises = Some (from, msg))
                    (GET_TGT: Cell.get to cell_tgt = Some (from, msg)),
           <<GET_SRC: Cell.get to cell_src = None>>)
       (COMPLETE2: forall to from msg
-                   (CAP: Some to <> cap)
                    (GETP: Cell.get to promises = None)
                    (GET_TGT: Cell.get to cell_tgt = Some (from, msg)),
           <<GET_SRC: Cell.get to cell_src = Some (from, msg)>>)
-      (LATEST: forall to (CAP: Some to = cap), Time.lt latest to)
-      (CAP: forall to (CAP: Some to = cap),
-          exists f val r from released,
-            <<LATEST: Cell.get latest cell_tgt = Some (f, Message.concrete val r)>> /\
-            <<CAP_SRC: Cell.get to cell_src = cap_src_cell latest promises from val released>> /\
-            <<CAP_TGT: Cell.get to cell_tgt = Some (from, Message.concrete val released)>> /\
-            <<CAPP: Cell.get to promises = None>>)
   .
 
-  Inductive sim_cell_aux (latest: Time.t) (cap: option Time.t) (dom: list Time.t) (promises cell_src cell_tgt: Cell.t): Prop :=
+  Inductive sim_cell_aux (dom: list Time.t) (promises cell_src cell_tgt: Cell.t): Prop :=
   | sim_cell_aux_intro
-      (LATEST: exists from val released,
-          Cell.get latest cell_tgt = Some (from, Message.concrete val released))
       (SOUND: Cell.le cell_src cell_tgt)
       (COMPLETE1: forall from to msg
-                    (CAP: Some to <> cap)
                     (GETP: Cell.get to promises = Some (from, msg))
                     (GET_TGT: Cell.get to cell_tgt = Some (from, msg)),
           <<GET_SRC: Cell.get to cell_src = None>>)
-      (COMPLETE2: forall from to val released
-                    (CAP: Some to <> cap)
+      (COMPLETE2: forall from to msg
+                    (IN: List.In to dom)
                     (GETP: Cell.get to promises = None)
-                    (GET_TGT: Cell.get to cell_tgt = Some (from, Message.concrete val released)),
-          <<GET_SRC: Cell.get to cell_src = Some (from, Message.concrete val released)>>)
-      (RESERVE: forall from to
-               (IN: List.In to dom)
-               (GETP: Cell.get to promises = None)
-               (GET_TGT: Cell.get to cell_tgt = Some (from, Message.reserve)),
-          <<GET_SRC: Cell.get to cell_src = Some (from, Message.reserve)>>)
-      (LATESTS: forall to (CAP: Some to = cap), Time.lt latest to)
-      (CAP: forall to (CAP: Some to = cap),
-          exists f val r from released,
-            <<LATEST: Cell.get latest cell_tgt = Some (f, Message.concrete val r)>> /\
-            <<CAP_SRC: List.In to dom /\
-                       Cell.get to cell_src = cap_src_cell latest promises from val released \/
-                       ~ List.In to dom /\
-                       Cell.get to cell_src = None>> /\
-            <<CAP_TGT: Cell.get to cell_tgt = Some (from, Message.concrete val released)>> /\
-            <<CAPP: Cell.get to promises = None>>)
-  .
-
-  Inductive cap_cell (promises cell1 cell2: Cell.t): Prop :=
-  | cap_cell_intro
-      latest
-      (LATEST: Cell.max_concrete_ts cell1 latest)
-      (SOUND: Cell.le cell1 cell2)
-      (MIDDLE: forall from1 to1 from2 to2
-                 (ADJ: Cell.adjacent from1 to1 from2 to2 cell1)
-                 (TS: Time.lt to1 from2),
-          Cell.get from2 cell2 = Some (to1, Message.reserve))
-      (BACK: forall to
-               (TO: to = Time.incr (Cell.max_ts cell1))
-               (PROMISE: Cell.latest_reserve promises cell1),
-          exists f val r released,
-            Cell.get latest cell1 = Some (f, Message.concrete val r) /\
-            Cell.get to cell2 = Some (Cell.max_ts cell1, Message.concrete val released))
-      (COMPLETE: forall from to msg
-                   (GET2: Cell.get to cell2 = Some (from, msg)),
-          <<GET1: Cell.get to cell1 = Some (from, msg)>> \/
-          <<GET1: Cell.get to cell1 = None>> /\
-          <<TS: Time.lt from to>> /\
-          <<MSG: msg = Message.reserve>> /\
-          (exists from1 to1, <<ADJ: Cell.adjacent from1 from to to1 cell1>>) \/
-          <<GET1: Cell.get to cell1 = None>> /\
-          <<FROM: from = Cell.max_ts cell1>> /\
-          <<TO: to = Time.incr (Cell.max_ts cell1)>> /\
-          <<PROMISE: Cell.latest_reserve promises cell1>>)
+                    (GET_TGT: Cell.get to cell_tgt = Some (from, msg)),
+          <<GET_SRC: Cell.get to cell_src = Some (from, msg)>>)
   .
 
   Definition vals_incl_cell (cell1 cell2: Cell.t): Prop :=
@@ -1232,321 +78,182 @@ Module PFCertify.
     ii. exploit H; eauto. i. des. eauto.
   Qed.
 
-  Lemma cap_cap_cell
-        promises mem1 mem2
-        (CAP: Memory.cap promises mem1 mem2)
-        (CLOSED: Memory.closed mem1):
-    forall loc, cap_cell (promises loc) (mem1 loc) (mem2 loc).
-  Proof.
-    exploit Memory.max_concrete_timemap_exists; try apply CLOSED. i. des.
-    dup CAP. inv CAP0.
-    econs; i; eauto.
-    - apply x0.
-    - ii. eauto.
-    - inv ADJ. eapply MIDDLE; eauto. econs; eauto.
-    - exploit (@Memory.latest_val_exists loc mem1); try apply CLOSED. i. des.
-      exploit BACK; eauto. i.
-      inv x1. specialize (x0 loc).
-      exploit Memory.max_concrete_ts_inj; [exact MAX|exact x0|..]. i. subst.
-      inv x0. des.
-      unfold Memory.get in GET. rewrite GET in *. inv GET0.
-      esplits; eauto.
-    - exploit Memory.cap_inv; eauto. i. des; eauto.
-      + subst. right. left.
-        inv x2. esplits; eauto. econs; eauto.
-      + subst. right. right. esplits; eauto.
-  Qed.
-
-  Lemma cap_exists promises mem loc:
-    exists (cap: option Time.t),
-      if cap
-      then Memory.latest_reserve loc promises mem /\
-           cap = Some (Time.incr (Memory.max_ts loc mem))
-      else ~ Memory.latest_reserve loc promises mem.
-  Proof.
-    destruct (@Memory.latest_reserve_dec loc promises mem).
-    - eexists (Some _). esplits; eauto.
-    - exists None. eauto.
-  Qed.
-
-  Lemma sim_cell_exists
-        promises mem1_src mem1_tgt mem2_tgt latests
-        (SIM: PFStep.sim_memory promises mem1_src mem1_tgt)
-        (LE_TGT: Memory.le promises mem1_tgt)
-        (FINITE_TGT: Memory.finite promises)
-        (CLOSED1_TGT: Memory.closed mem1_tgt)
-        (CLOSED2_TGT: Memory.closed mem2_tgt)
-        (CAP: Memory.cap promises mem1_tgt mem2_tgt)
-        (MAX: Memory.max_concrete_timemap mem1_tgt latests):
-    forall loc,
-    exists cap cell_src,
-      sim_cell (latests loc) cap (promises loc) cell_src (mem2_tgt loc) /\
-      vals_incl_cell cell_src (mem1_src loc).
-  Proof.
-    i.
-    destruct (Cell.finite (mem2_tgt loc)).
-    rename x into dom.
-    destruct (@cap_exists promises mem1_tgt loc).
-    rename x into cap.
-    cut (exists cell_src,
-            sim_cell_aux (latests loc) cap dom (promises loc) cell_src (mem2_tgt loc) /\
-            vals_incl_cell cell_src (mem1_src loc)).
-    { i. des.
-      exists cap. exists cell_src. split; auto.
-      inv H1. econs; ii; eauto.
-      - destruct msg; eauto.
-      - exploit CAP0; eauto. i. des.
-        + esplits; eauto.
-        + exploit H; eauto. i. ss.
-    }
-    clear H. induction dom.
-    { exists (mem1_src loc). split; try refl.
-      exploit cap_cap_cell; eauto. i.
-      instantiate (1 := loc) in x0.
-      inv SIM. inv x0.
-      specialize (MAX loc).
-      exploit Memory.max_concrete_ts_inj; [exact MAX|apply LATEST|..]. i. subst.
-      econs; ii; eauto.
-      - inv MAX. des. exploit SOUND0; eauto.
-      - eapply COMPLETE1; eauto.
-      - exploit COMPLETE; eauto. i. des; eauto; ss.
-        subst. destruct cap; ss.
-        des. inv H1. ss.
-      - inv IN.
-      - rewrite <- CAP0 in *. des. inv H1.
-        inv LATEST. des.
-        exploit Cell.max_ts_spec; eauto. i. des.
-        eapply TimeFacts.le_lt_lt; eauto.
-        apply Time.incr_spec.
-      - rewrite <- CAP0 in *. des. inv H1.
-        inv LATEST. des.
-        destruct (Memory.get loc (Time.incr (Memory.max_ts loc mem1_tgt)) mem1_tgt) as [[]|] eqn:GETT.
-        { exploit Memory.max_ts_spec; try exact GETT. i. des.
-          specialize (Time.incr_spec (Memory.max_ts loc mem1_tgt)). i.
-          timetac. }
-        exploit BACK; eauto. i. des.
-        esplits; eauto.
-        + right. split; ss.
-          destruct (Memory.get loc (Time.incr (Memory.max_ts loc mem1_tgt)) mem1_src) as [[]|] eqn:GETS; ss.
-          exploit SOUND; eauto. i. congr.
-        + destruct (Memory.get loc (Time.incr (Memory.max_ts loc mem1_tgt)) promises) as [[]|] eqn:GETP; ss.
-          exploit LE_TGT; eauto. i. congr.
-    }
-    des. rename a into to.
-    destruct (In_decidable time_decidable to dom).
-    { exists cell_src. split; auto.
-      inv IHdom. econs; ii; eauto; ss.
-      - inv IN; eauto.
-      - exploit CAP0; eauto. i. des.
-        + esplits; eauto.
-        + esplits; eauto. right. split; ss.
-          ii. des; ss. inv H1. ss.
-    }
-    destruct (Cell.get to (mem2_tgt loc)) as [[]|] eqn:GETT; cycle 1.
-    { exists cell_src. split; auto.
-      inv IHdom. econs; ii; eauto; ss.
-      - inv IN; eauto. congr.
-      - exploit CAP0; eauto. i. des; esplits; eauto.
-        right. split; ss.
-        ii. des; ss. inv H1. congr.
-    }
-    destruct (Cell.get to cell_src) as [[]|] eqn:GETS.
-    { exists cell_src. split; auto.
-      inv IHdom. exploit SOUND; eauto. i.
-      rewrite GETT in *. inv x.
-      econs; ii; eauto; ss.
-      - inv IN; eauto.
-        rewrite GET_TGT in *. inv GETT. ss.
-      - exploit CAP0; eauto. i. des; esplits; eauto.
-        right. split; ss. ii. des; ss.
-        inv H1. congr.
-    }
-    destruct (Cell.get to (promises loc)) as [[]|] eqn:GETP.
-    { exists cell_src. split; auto.
-      inv IHdom. econs; ii; eauto; ss.
-      - inv IN; eauto. congr.
-      - exploit CAP0; eauto. i. des; esplits; eauto.
-        right. split; ss. ii. des; ss. inv H1. congr.
-    }
-    destruct (opt_ts_eq_dec cap (Some to)); cycle 1.
-    { destruct t0.
-      { exists cell_src. split; auto.
-        inv IHdom. econs; ii; eauto; ss.
-        - inv IN; eauto.
-          exploit COMPLETE2; eauto. i. congr.
-        - exploit CAP0; eauto. i. des; esplits; eauto.
-          right. split; ss. ii. des; ss. inv H1. congr.
-      }
-      exploit (@Cell.add_exists cell_src t to Message.reserve).
-      { ii. inv IHdom.
-        exploit SOUND; try exact GET2. i.
-        exploit Cell.get_disjoint; [exact GETT|exact x0|..]. i. des.
-        - subst. congr.
-        - eapply x2; eauto. }
-      { exploit Cell.get_ts; try exact GETT. i. des; ss.
-        subst. inv CLOSED1_TGT. specialize (INHABITED loc).
-        inv CAP. exploit SOUND; try exact INHABITED. i.
-        unfold Memory.get in *. rewrite x in *. inv GETT. }
-      { econs. }
-      i. des.
-      exists cell2.
-      split; cycle 1.
-      { etrans; eauto. ii. revert GET1.
-        erewrite Cell.add_o; eauto. condtac; ss; eauto. }
-      inv IHdom. econs; ii; eauto; ss.
-      - revert LHS.
-        erewrite Cell.add_o; eauto. condtac; ss; eauto.
-        i. des. subst. inv LHS. ss.
-      - erewrite Cell.add_o; eauto. condtac; ss; eauto.
-        des. subst. congr.
-      - erewrite Cell.add_o; eauto. condtac; ss; eauto.
-        des. subst. congr.
-      - erewrite Cell.add_o; eauto. condtac; ss; eauto.
-        + des; subst; ss.
-          rewrite GETT in *. inv GET_TGT. ss.
-        + guardH n0. des; eauto. inv IN. unguard. des; ss.
-      - exploit CAP0; eauto. i. des; esplits; eauto.
-        + left. split; eauto.
-          erewrite Cell.add_o; eauto. condtac; ss; eauto.
-          des. subst. congr.
-        + right. split.
-          * ii. des; ss. inv H1; eauto.
-          * erewrite Cell.add_o; eauto. condtac; ss.
-            des. subst. congr.
-    }
-    rewrite e in *. des. inv H1.
-    exploit cap_cap_cell; eauto. i.
-    instantiate (1 := loc) in x0. inv x0.
-    exploit BACK; eauto. i. des.
-    exploit Cell.max_concrete_ts_inj; [eapply MAX|exact LATEST|..]. i. subst.
-    clear LATEST SOUND MIDDLE BACK COMPLETE.
-    unfold Memory.max_ts in *. rewrite GETT in *. inv x0.
-    destruct (Cell.get (latests loc) (promises loc)) as [[]|] eqn:LATESTP.
-    { exploit LE_TGT; try exact LATESTP. i.
-      unfold Memory.get in *. rewrite x in *. inv x0.
-      exists cell_src. split; auto.
-      inv IHdom. econs; ii; eauto; ss.
-      - inv IN; eauto. congr.
-      - exploit CAP0; eauto. i. des; esplits; eauto.
-        left. inv CAP1. split; eauto.
-        unfold cap_src_cell. rewrite LATESTP. ss.
-    }
-    exploit (@Cell.add_exists cell_src (Cell.max_ts (mem1_tgt loc))
-                              (Time.incr (Cell.max_ts (mem1_tgt loc))) (Message.concrete val released)).
-    { ii. inv IHdom. exploit SOUND; try exact GET2. i.
-      exploit Memory.get_disjoint; [exact GETT|exact x1|..]. i. des.
-      - subst. congr.
-      - eapply x3; eauto. }
-    { apply Time.incr_spec. }
-    { inv CLOSED2_TGT. exploit CLOSED; try exact GETT. i. des. ss. }
-    i. des.
-    exists cell2.
-    split; cycle 1.
-    { etrans; eauto. ii. revert GET1.
-      erewrite Cell.add_o; eauto. condtac; ss; eauto. i.
-      des. subst. inv GET1.
-      inv CAP. exploit SOUND; try exact x. i.
-      inv IHdom. exploit COMPLETE2; try exact x0; eauto.
-      ii. exploit LATESTS; eauto. i. timetac. }
-    inv IHdom. econs; ii; eauto; ss.
-    - revert LHS.
-      erewrite Cell.add_o; eauto. condtac; ss; eauto.
-      i. des. subst. inv LHS. ss.
-    - erewrite Cell.add_o; eauto. condtac; ss; eauto.
-      des. subst. congr.
-    - erewrite Cell.add_o; eauto. condtac; ss; eauto.
-      des. subst. congr.
-    - erewrite Cell.add_o; eauto. condtac; ss.
-      + des; subst; ss. congr.
-      + guardH n. des; eauto. inv IN. unguard. des; ss.
-    - exploit CAP0; eauto. i. des; esplits; eauto.
-      + left. split; eauto.
-        erewrite Cell.add_o; eauto. condtac; ss; eauto.
-        des. subst. ss.
-      + left. inv CAP1. split; eauto.
-        rewrite GETT in *. inv CAP_TGT.
-        unfold cap_src_cell. rewrite LATESTP.
-        exploit Cell.add_get0; eauto. i. des. ss.
-  Qed.
-
-  Lemma sim_memory_exists
+  Lemma cap_sim_cell_exists
         promises mem1_src mem1_tgt mem2_tgt
         (SIM: PFStep.sim_memory promises mem1_src mem1_tgt)
         (LE_TGT: Memory.le promises mem1_tgt)
         (FINITE_TGT: Memory.finite promises)
         (CLOSED1_TGT: Memory.closed mem1_tgt)
         (CLOSED2_TGT: Memory.closed mem2_tgt)
-        (CAP: Memory.cap promises mem1_tgt mem2_tgt):
-    exists latests caps mem2_src,
-      sim_memory latests caps promises mem2_src mem2_tgt /\
+        (CAP: Memory.cap mem1_tgt mem2_tgt):
+    forall loc,
+    exists cell_src,
+      sim_cell (promises loc) cell_src (mem2_tgt loc) /\
+      vals_incl_cell cell_src (mem1_src loc) /\
+      Cell.le (mem1_src loc) cell_src.
+  Proof.
+    i.
+    destruct (Cell.finite (mem2_tgt loc)).
+    rename x into dom.
+    cut (exists cell_src,
+            sim_cell_aux dom (promises loc) cell_src (mem2_tgt loc) /\
+            vals_incl_cell cell_src (mem1_src loc) /\
+            Cell.le (mem1_src loc) cell_src).
+    { i. des.
+      exists cell_src. splits; auto.
+      inv H0. econs; ii; eauto.
+    }
+    clear H. induction dom.
+    { exists (mem1_src loc). splits; try refl.
+      inv SIM. inv CAP. econs; ii; eauto.
+      - eapply COMPLETE1; eauto.
+      - ss.
+    }
+    des. rename a into to.
+    destruct (In_decidable time_decidable to dom).
+    { exists cell_src. splits; auto.
+      inv IHdom. econs; ii; eauto; ss.
+      inv IN; eauto.
+    }
+    destruct (Cell.get to (mem2_tgt loc)) as [[]|] eqn:GETT; cycle 1.
+    { exists cell_src. splits; auto.
+      inv IHdom. econs; ii; eauto; ss.
+      inv IN; eauto. congr.
+    }
+    destruct (Cell.get to cell_src) as [[]|] eqn:GETS.
+    { exists cell_src. splits; auto.
+      inv IHdom. exploit SOUND; eauto. i.
+      rewrite GETT in *. inv x.
+      econs; ii; eauto; ss.
+      inv IN; eauto.
+      rewrite GET_TGT in *. inv GETT. ss.
+    }
+    destruct (Cell.get to (promises loc)) as [[]|] eqn:GETP.
+    { exists cell_src. splits; auto.
+      inv IHdom. econs; ii; eauto; ss.
+      inv IN; eauto. congr.
+    }
+    destruct (Cell.get to (mem1_tgt loc)) as [[]|] eqn:GETT1.
+    { inv SIM. exploit COMPLETE2; eauto. i. des.
+      exploit IHdom1; eauto. i. congr.
+    }
+    exploit Memory.cap_inv; try exact CAP; eauto. i. des.
+    { unfold Memory.get in *. congr. }
+    { subst. clear x0.
+      exploit (@Cell.add_exists cell_src t to Message.reserve).
+      { ii. inv IHdom.
+        exploit SOUND; try exact GET2. i.
+        exploit Cell.get_disjoint; [exact GETT|exact x0|..]. i. des.
+        - subst. congr.
+        - eapply x4; eauto. }
+      { exploit Cell.get_ts; try exact GETT. i. des; ss. }
+      { econs. }
+      i. des.
+      exists cell2.
+      splits; cycle 1.
+      { etrans; eauto. ii. revert GET1.
+        erewrite Cell.add_o; eauto. condtac; ss; eauto. }
+      { ii. exploit Cell.add_get1; try exact x0; eauto. }
+      inv IHdom. econs; ii; eauto; ss.
+      - revert LHS.
+        erewrite Cell.add_o; eauto. condtac; ss; eauto.
+        i. des. subst. inv LHS. ss.
+      - erewrite Cell.add_o; eauto. condtac; ss; eauto.
+        des. subst. congr.
+      - des.
+        + subst. rewrite GET_TGT in *. inv GETT.
+          erewrite Cell.add_o; eauto. condtac; ss.
+        + exploit COMPLETE2; eauto. i. des.
+          eapply Cell.add_get1; eauto.
+    }
+    { subst. clear x0.
+      exploit (@Cell.add_exists cell_src (Memory.max_ts loc mem1_tgt)
+                                (Time.incr (Memory.max_ts loc mem1_tgt)) Message.reserve).
+      { ii. inv IHdom. exploit SOUND; try exact GET2. i.
+        exploit Memory.get_disjoint; [exact GETT|exact x0|..]. i. des.
+        - subst. congr.
+        - eapply x2; eauto. }
+      { apply Time.incr_spec. }
+      { inv CLOSED2_TGT. exploit CLOSED; try exact GETT. i. des. ss. }
+      i. des.
+      exists cell2.
+      splits; cycle 1.
+      { etrans; eauto. ii. revert GET1.
+        erewrite Cell.add_o; eauto. condtac; ss; eauto. }
+      { ii. exploit IHdom1; eauto. i.
+        eapply Cell.add_get1; eauto. }
+      { inv IHdom. econs; ii; eauto; ss.
+        - revert LHS.
+          erewrite Cell.add_o; eauto. condtac; ss; eauto.
+          i. des. subst. inv LHS. ss.
+        - erewrite Cell.add_o; eauto. condtac; ss; eauto.
+          des. subst. congr.
+        - des.
+          + subst. rewrite GET_TGT in *. inv GETT.
+            erewrite Cell.add_o; eauto. condtac; ss.
+          + exploit COMPLETE2; eauto. i. des.
+            eapply Cell.add_get1; eauto. }
+    }
+  Qed.
+
+  Lemma cap_sim_memory_exists
+        promises mem1_src mem1_tgt mem2_tgt
+        (SIM: sim_memory promises mem1_src mem1_tgt)
+        (LE_TGT: Memory.le promises mem1_tgt)
+        (FINITE_TGT: Memory.finite promises)
+        (CLOSED1_TGT: Memory.closed mem1_tgt)
+        (CLOSED2_TGT: Memory.closed mem2_tgt)
+        (CAP: Memory.cap mem1_tgt mem2_tgt):
+    exists mem2_src,
+      sim_memory promises mem2_src mem2_tgt /\
       vals_incl mem2_src mem1_src.
   Proof.
-    exploit Memory.max_concrete_timemap_exists; try apply CLOSED1_TGT. i. des.
-    exists tm.
-    cut (exists (caps_mem: Loc.t -> ((option Time.t) * Cell.t)),
+    cut (exists (caps_mem: Loc.t -> Cell.t),
             forall loc,
               (fun loc cap_cell =>
-                 sim_cell (tm loc) cap_cell.(fst) (promises loc) cap_cell.(snd) (mem2_tgt loc) /\
-                 vals_incl_cell cap_cell.(snd) (mem1_src loc))
+                 sim_cell (promises loc) cap_cell (mem2_tgt loc) /\
+                 vals_incl_cell cap_cell (mem1_src loc))
                 loc (caps_mem loc)).
     { i. des.
-      exists (fun loc => (caps_mem loc).(fst)).
-      exists (fun loc => (caps_mem loc).(snd)).
+      exists (fun loc => caps_mem loc).
       split.
       - econs; ii; eauto.
         + destruct (H loc). inv H0. eauto.
         + destruct (H loc). inv H0. eapply COMPLETE1; eauto.
         + destruct (H loc). inv H0. eauto.
-        + destruct (H loc). inv H0.
-          exploit LATEST0; eauto.
-        + destruct (H loc). inv H0. eauto.
       - ii. destruct (H loc). eauto.
     }
     apply choice. intro loc.
-    exploit sim_cell_exists; eauto. i. des.
+    exploit cap_sim_cell_exists; eauto. i. des.
     instantiate (1 := loc) in x1.
-    exists (cap, cell_src). ss.
+    exists cell_src. ss.
   Qed.
 
-  Lemma sim_thread_exists
+  Lemma cap_sim_thread_exists
         lang e_src e_tgt
         sc1 mem1_tgt
-        (SIM: @PFStep.sim_thread lang e_src e_tgt)
+        (SIM: @sim_thread lang e_src e_tgt)
         (WF1_TGT: Local.wf e_tgt.(Thread.local) e_tgt.(Thread.memory))
         (SC1_TGT: Memory.closed_timemap e_tgt.(Thread.sc) e_tgt.(Thread.memory))
         (MEM1_TGT: Memory.closed e_tgt.(Thread.memory))
         (SC_TGT: Memory.max_concrete_timemap mem1_tgt sc1)
-        (CAP_TGT: Memory.cap e_tgt.(Thread.local).(Local.promises) e_tgt.(Thread.memory) mem1_tgt):
-    exists latests caps mem1_src,
-      <<SIM: sim_thread latests caps
-                        (Thread.mk lang e_src.(Thread.state) e_src.(Thread.local) sc1 mem1_src)
+        (CAP_TGT: Memory.cap e_tgt.(Thread.memory) mem1_tgt):
+    exists mem1_src,
+      <<SIM: sim_thread (Thread.mk lang e_src.(Thread.state) e_src.(Thread.local) sc1 mem1_src)
                         (Thread.mk lang e_tgt.(Thread.state) e_tgt.(Thread.local) sc1 mem1_tgt)>> /\
       <<VALS: vals_incl mem1_src e_src.(Thread.memory)>>.
   Proof.
     exploit Memory.cap_closed; eauto. i.
-    exploit sim_memory_exists; try apply SIM; try apply WF1_TGT; eauto. i. des.
+    exploit cap_sim_memory_exists; try apply SIM; try apply WF1_TGT; eauto. i. des.
     esplits; eauto.
     econs; eauto.
     - inv SIM. ss.
     - inv SIM. ss.
   Qed.
 
-  Lemma sim_memory_inhabited
-        latests caps promises mem_src mem_tgt
-        (SIM: sim_memory latests caps promises mem_src mem_tgt)
-        (BOT: Memory.bot_none promises)
-        (INHABITED_TGT: Memory.inhabited mem_tgt):
-    <<INHABITED_SRC: Memory.inhabited mem_src>>.
-  Proof.
-    inv SIM. ii.
-    specialize (BOT loc). specialize (INHABITED_TGT loc).
-    exploit COMPLETE2; eauto. ii.
-    exploit LATESTS; eauto. i. inv x.
-  Qed.
-
   Lemma sim_memory_bot
-        latests caps promises mem_src mem_tgt
-        (SIM: sim_memory latests caps promises mem_src mem_tgt)
+        promises mem_src mem_tgt
+        (SIM: sim_memory promises mem_src mem_tgt)
         (PROMISES: promises = Memory.bot):
     mem_src = mem_tgt.
   Proof.
@@ -1554,11 +261,7 @@ Module PFCertify.
     destruct (Memory.get loc ts mem_src) as [[]|] eqn:GETS.
     { exploit SOUND; eauto. }
     destruct (Memory.get loc ts mem_tgt) as [[]|] eqn:GETT; ss.
-    destruct (opt_ts_eq_dec (Some ts) (caps loc)).
-    - exploit CAPS; eauto. i. des.
-      unfold cap_src in *. rewrite Memory.bot_get in *.
-      congr.
-    - exploit COMPLETE2; eauto; try congr.
-      apply Memory.bot_get.
+    exploit COMPLETE2; eauto; try congr.
+    apply Memory.bot_get.
   Qed.
 End PFCertify.
