Makefile
@@ -5,10 +5,10 @@ COQTHEORIES  := \
 	src/while/*.v \
 	src/prop/*.v \
 	src/opt/*.v \
-#	src/pf/*.v \
-#	src/invariant/*.v \
+	src/invariant/*.v \
 #	src/gopt/*.v \
 #	src/promotion/*.v \
+#	src/pf/*.v \
 #	src/drf/*.v
 
 .PHONY: all theories clean
@@ -27,10 +27,10 @@ Makefile.coq: Makefile $(COQTHEORIES)
    echo "-R src/while $(COQMODULE)"; \
    echo "-R src/prop $(COQMODULE)"; \
    echo "-R src/opt $(COQMODULE)"; \
-#   echo "-R src/pf $(COQMODULE)"; \
-#   echo "-R src/invariant $(COQMODULE)"; \
+   echo "-R src/invariant $(COQMODULE)"; \
 #   echo "-R src/gopt $(COQMODULE)"; \
 #   echo "-R src/promotion $(COQMODULE)"; \
+#   echo "-R src/pf $(COQMODULE)"; \
 #   echo "-R src/drf $(COQMODULE)"; \
    \
    echo $(COQTHEORIES)) > _CoqProject
